updated Salsa spec and fixed ct coercions

code/salsa-family/Hacl.Impl.Chacha20.fst
@@ -30,127 +30,6 @@ private inline_for_extraction let op_Less_Less_Less (a:h32) (s:u32{U32.v s <= 32
 
 #reset-options "--initial_fuel 0 --max_fuel 0 --z3rlimit 100"
 
-(* private val lemma_uint32s_from_le_bytes: h:mem -> output:buffer H32.t{live h output} -> *)
-(*   h':mem -> input:uint8_p{live h' input} -> *)
-(*   len:U32.t{length output = U32.v len /\ 4 * U32.v len = length input /\ U32.v len > 0} -> *)
-(*   Lemma *)
-(*     (requires (H32.v (Seq.index (as_seq h output) 0) = *)
-(*         U32.v (Spec.Lib.uint32_from_le (reveal_sbytes (as_seq h' (Buffer.sub input 0ul 4ul)))) *)
-(*       /\ reveal_h32s (as_seq h (Buffer.offset output 1ul)) ==  *)
-(*         Spec.Lib.uint32s_from_le (UInt32.v len - 1) (reveal_sbytes (as_seq h' (Buffer.offset input 4ul))))) *)
-(*     (ensures (reveal_h32s (as_seq h output) *)
-(*       == Spec.Lib.uint32s_from_le (U32.v len) (reveal_sbytes ((as_seq h' input))))) *)
-(* let lemma_uint32s_from_le_bytes h output h' input len = *)
-(*   let i' = reveal_sbytes (as_seq h' input) in *)
-(*   Spec.Lib.lemma_uint32s_from_le_def_1 (U32.v len) i'; *)
-(*   Seq.lemma_eq_intro (as_seq h' (Buffer.sub input 0ul 4ul)) (Seq.slice (as_seq h' input) 0 4); *)
-(*   Seq.lemma_eq_intro (as_seq h' (Buffer.offset input 4ul)) (Seq.slice (as_seq h' input) 4 (length input)); *)
-(*   Seq.lemma_eq_intro (as_seq h (Buffer.offset output 1ul)) (Seq.slice (as_seq h output) 1 (length output)); *)
-(*   cut (Seq.index (Spec.Lib.uint32s_from_le (U32.v len) i') 0 == Spec.Lib.uint32_from_le (Seq.slice i' 0 4)); *)
-(*   Seq.lemma_eq_intro (reveal_h32s (as_seq h output)) (Spec.Lib.uint32s_from_le (U32.v len) i') *)
-
-
-(* private val lemma_uint32s_from_le_bytes': h:mem -> h':mem -> output:buffer H32.t{live h output /\ live h' output /\ length output > 0} -> Lemma *)
-(*   (requires (modifies_1 (Buffer.offset output 1ul) h h')) *)
-(*   (ensures (Seq.index (as_seq h output) 0 == Seq.index (as_seq h' output) 0)) *)
-(* private let lemma_uint32s_from_le_bytes' h h' output = *)
-(*   let output' = Buffer.sub output 0ul 1ul in *)
-(*   let output'' = Buffer.offset output 1ul in *)
-(*   no_upd_lemma_1 h h' output'' output'; *)
-(*   Seq.lemma_eq_intro (Seq.slice (as_seq h output) 0 1) (as_seq h output'); *)
-(*   Seq.lemma_eq_intro (Seq.append (as_seq h' output') (as_seq h' output'')) (as_seq h' output) *)
-
-
-(* val uint32s_from_le_bytes: *)
-(*   output:buffer H32.t -> *)
-(*   input:uint8_p{disjoint output input} -> *)
-(*   len:U32.t{length output = U32.v len /\ 4 * U32.v len = length input} -> *)
-(*   Stack unit *)
-(*     (requires (fun h -> live h output /\ live h input)) *)
-(*     (ensures  (fun h0 _ h1 -> live h1 output /\ live h0 input /\ modifies_1 output h0 h1 /\ *)
-(*       (let o = reveal_h32s (as_seq h1 output) in *)
-(*        let i = reveal_sbytes (as_seq h0 input) in *)
-(*        o == Spec.Lib.uint32s_from_le (U32.v len) i))) *)
-(* let rec uint32s_from_le_bytes output input len = *)
-(*   let h0 = ST.get() in *)
-(*   if U32.(len =^ 0ul) then ( *)
-(*     Spec.Lib.lemma_uint32s_from_le_def_0 0 (reveal_sbytes (as_seq h0 input)); *)
-(*     Seq.lemma_eq_intro (as_seq h0 output) Seq.createEmpty *)
-(*   ) *)
-(*   else ( *)
-(*     cut (U32.v len > 0); *)
-(*     output.(0ul) <- hload32_le (Buffer.sub input 0ul 4ul); *)
-(*     let h = ST.get() in *)
-(*     let output' = Buffer.offset output 1ul in *)
-(*     let input'  = Buffer.offset input 4ul in *)
-(*     uint32s_from_le_bytes output' input' U32.(len -^ 1ul); *)
-(*     let h1 = ST.get() in *)
-(*     lemma_uint32s_from_le_bytes' h h1 output; *)
-(*     lemma_uint32s_from_le_bytes h1 output h0 input len *)
-(*   ) *)
-
-
-(* private val lemma_uint32s_to_le_bytes: h:mem -> output:uint8_p{live h output} -> *)
-(*   h':mem -> input:buffer H32.t{live h' input} -> *)
-(*   len:U32.t{length input = U32.v len /\ 4 * U32.v len = length output /\ U32.v len > 0} -> *)
-(*   Lemma *)
-(*     (requires (Seq.slice (reveal_sbytes (as_seq h output)) 0 4 = Spec.Lib.uint32_to_le (Seq.index (reveal_h32s (as_seq h' input)) 0) *)
-(*       /\ reveal_sbytes (as_seq h (Buffer.offset output 4ul)) == Spec.Lib.uint32s_to_le (UInt32.v len - 1) (reveal_h32s (as_seq h' (Buffer.offset input 1ul))))) *)
-(*     (ensures (reveal_sbytes (as_seq h output) == Spec.Lib.uint32s_to_le (U32.v len) (reveal_h32s ((as_seq h' input))))) *)
-(* let lemma_uint32s_to_le_bytes h output h' input len = *)
-(*   let i' = reveal_h32s (as_seq h' input) in *)
-(*   Spec.Lib.lemma_uint32s_to_le_def_1 (U32.v len) i'; *)
-(*   Seq.lemma_eq_intro (as_seq h (Buffer.sub output 0ul 4ul)) (Seq.slice (as_seq h output) 0 4); *)
-(*   Seq.lemma_eq_intro (as_seq h (Buffer.offset output 4ul)) (Seq.slice (as_seq h output) 4 (length output)); *)
-(*   Seq.lemma_eq_intro (as_seq h' (Buffer.offset input 1ul)) (Seq.slice (as_seq h' input) 1 (length input)); *)
-(*   Seq.lemma_eq_intro (Seq.slice (Spec.Lib.uint32s_to_le (U32.v len) i') 0 4) *)
-(*                      (Spec.Lib.uint32_to_le (Seq.index i' 0)); *)
-(*   Seq.lemma_eq_intro (reveal_sbytes (as_seq h output)) (Spec.Lib.uint32s_to_le (U32.v len) i') *)
-
-
-(* private val lemma_uint32s_to_le_bytes': h:mem -> h':mem -> output:uint8_p{live h output /\ live h' output /\ length output >= 4} -> Lemma *)
-(*   (requires (modifies_1 (Buffer.offset output 4ul) h h')) *)
-(*   (ensures (Seq.slice (as_seq h output) 0 4 == Seq.slice (as_seq h' output) 0 4)) *)
-(* private let lemma_uint32s_to_le_bytes' h h' output = *)
-(*   let output' = Buffer.sub output 0ul 4ul in *)
-(*   let output'' = Buffer.offset output 4ul in *)
-(*   no_upd_lemma_1 h h' output'' output'; *)
-(*   Seq.lemma_eq_intro (Seq.slice (as_seq h output) 0 4) (as_seq h output') *)
-
-
-(* val uint32s_to_le_bytes: *)
-(*   output:uint8_p -> *)
-(*   input:buffer H32.t{disjoint output input} -> *)
-(*   len:U32.t{length input = U32.v len /\ 4 * U32.v len = length output} -> *)
-(*   Stack unit *)
-(*     (requires (fun h -> live h output /\ live h input)) *)
-(*     (ensures  (fun h0 _ h1 -> live h1 output /\ live h0 input /\ modifies_1 output h0 h1 /\ *)
-(*       (let o = reveal_sbytes (as_seq h1 output) in *)
-(*        let i = reveal_h32s (as_seq h0 input) in *)
-(*        o == Spec.Lib.uint32s_to_le (U32.v len) i))) *)
-(* let rec uint32s_to_le_bytes output input len = *)
-(*   let h0 = ST.get() in *)
-(*   if U32.(len =^ 0ul) then ( *)
-(*     Spec.Lib.lemma_uint32s_to_le_def_0 0 (reveal_h32s (as_seq h0 input)); *)
-(*     Seq.lemma_eq_intro (as_seq h0 output) Seq.createEmpty *)
-(*   ) *)
-(*   else ( *)
-(*     cut (U32.v len > 0); *)
-(*     let hd = input.(0ul) in *)
-(*     hstore32_le (Buffer.sub output 0ul 4ul) hd; *)
-(*     let h = ST.get() in *)
-(*     FStar.Endianness.lemma_little_endian_inj (Seq.slice (reveal_sbytes (as_seq h output)) 0 4) *)
-(*                                              (Spec.Lib.uint32_to_le (h32_to_u32 hd)); *)
-(*     cut (Seq.slice (reveal_sbytes (as_seq h output)) 0 4 == Spec.Lib.uint32_to_le (h32_to_u32 hd)); *)
-(*     let output' = Buffer.offset output 4ul in *)
-(*     let input'  = Buffer.offset input 1ul in *)
-(*     uint32s_to_le_bytes output' input' U32.(len -^ 1ul); *)
-(*     let h1 = ST.get() in *)
-(*     lemma_uint32s_to_le_bytes' h h1 output; *)
-(*     lemma_uint32s_to_le_bytes h1 output h0 input len *)
-(*   ) *)
-
-
 #reset-options "--initial_fuel 0 --max_fuel 0 --initial_ifuel 0 --max_ifuel 0 --z3rlimit 100"
 
 [@ "substitute"]
@@ -378,12 +257,6 @@ let double_round st =
     diagonal_round st
 
 
-(* unfold inline_for_extraction *)
-(* let double_round' (b:Seq.seq H32.t{Seq.length b = 16}) : Tot (b':Seq.seq H32.t{Seq.length b' = Seq.length b /\ reveal_h32s b' == Spec.Chacha20.double_round (reveal_h32s b)}) = *)
-(*   let f (s:Seq.seq U32.t{Seq.length s = 16}) : Tot (s':Seq.seq U32.t{Seq.length s' = 16}) = Spec.Chacha20.double_round s in *)
-(*   lift_32 #(fun s -> Seq.length s = 16) f b *)
-
-
 #reset-options "--initial_fuel 0 --max_fuel 0 --z3rlimit 500"
 
 [@ "c_inline"]
@@ -409,7 +282,7 @@ let rounds st =
   = double_round st;
     Spec.Loops.lemma_repeat (UInt32.v i + 1) Spec.Chacha20.double_round (reveal_h32s (as_seq h0 st))
   in
-  lemma_repeat_0 0 Spec.Chacha20.double_round (as_seq h0 st);
+  lemma_repeat_0 0 Spec.Chacha20.double_round (reveal_h32s (as_seq h0 st));
   for 0ul 10ul inv f'
 
 
