specs/Spec.Salsa20.fst
@@ -49,7 +49,7 @@ let row_round : shuffle =
 let double_round: shuffle = 
   column_round @ row_round (* 2 rounds *)
 
-let rec rounds : shuffle = 
+let rounds : shuffle = 
     Spec.Loops.repeat_spec 10 double_round (* 20 rounds *)
 
 let salsa20_core (s:state) : Tot state = 
